all compile errors resolved

peterson.dfy
@@ -1,86 +1,92 @@
-datatype Process = 0 | 1;
-datatype CState =  a1 | a2 | a3a | a3b | cs | a4;
-datatype State = State(pc: Process -> CState, flag: Process -> bool, turn: Process)
+type Process = nat
+datatype CState =  a1 | a2 | a3a | a3b | cs | a4
+datatype State = State(pc: map<Process, CState>, flag: map<Process, bool>, turn: Process)
 
-const P : set <Process>
+predicate ValidProcess(p: Process) {
+    p == 0 || p == 1
+}
 
-function Other(p: process) : Process
+function Other(p: Process) : (q: Process)
+requires ValidProcess(p)
+ensures ValidProcess(q)
 {
     if p == 0 then 1 else 0
 }
 
 predicate Valid(s: State) {
-    s.flag.Keys == s.pc.Keys == P
+    (forall p :: p in s.flag.Keys && ValidProcess(p)) &&
+    forall p :: p in s.pc.Keys && ValidProcess(p)
 }
 
 predicate Init(s: State) {
-    s.flag(0) == s.flag(1) == false &&
+    Valid(s) &&
+    s.flag[0] == s.flag[1] == false &&
     s.turn == 0 &&
-    s.pc(0) == s.pc(1) == a1
+    s.pc[0] == a1 && s.pc[1] == a1
 }
 
 predicate Next(s: State, s': State) {
     Valid(s) &&
-    exists p : Process :: p in P && NextP(p, s, s')
+    exists p : Process :: ValidProcess(p) && NextP(p, s, s')
 }
 
 predicate NextP(p: Process, s: State, s': State)
-requires Valid(s) && p in P
+requires Valid(s) && ValidProcess(p)
 {
-    a1(p, s, s') ||
-    a2(p, s, s') ||
-    a3a(p, s, s') ||
-    a3b(p, s, s') ||
-    cs(p, s, s') ||
-    a4(p, s, s')
+    (s.pc[p] == a1 && stmt_a1(p, s, s')) ||
+    (s.pc[p] == a2 && stmt_a2(p, s, s')) ||
+    (s.pc[p] == a3a && stmt_a3a(p, s, s')) ||
+    (s.pc[p] == a3b && stmt_a3b(p, s, s')) ||
+    (s.pc[p] == cs && stmt_cs(p, s, s')) ||
+    (s.pc[p] == a4 && stmt_a4(p, s, s'))
 }
 
-predicate a1(p: Process, s: State, s': State) 
-requires p in P && Valid(s) && s.pc(p) == a1
+predicate stmt_a1(p: Process, s: State, s': State) 
+requires ValidProcess(p) && Valid(s) && s.pc[p] == a1
 {
-    s'.flag(p) == true &&
-    s'.pc(p) == a2
+    s'.flag == s.flag[p := true] &&
+    s'.pc == s.pc[p := a2]
 }
 
-predicate a2(p: Process, s: State, s': State) 
-requires p in P && Valid(s) && s.pc(p) == a2
+predicate stmt_a2(p: Process, s: State, s': State) 
+requires ValidProcess(p) && Valid(s) && s.pc[p] == a2
 {
     s'.turn == Other(p) &&
-    s'.pc(p) == a3a;
+    s'.pc == s.pc[p := a3a]
 }
 
-method a3a(p: Process, s: State, s': State) 
-requires p in P && Valid(s) && s.pc(p) == a3a
+predicate stmt_a3a(p: Process, s: State, s': State) 
+requires ValidProcess(p) && Valid(s) && s.pc[p] == a3a
 {
-    (s.flag(Other(p)) && s'.pc(p) == a3b) ||
-    (!s.flag(Other(p)) && s'.pc(p) == cs)
+    (s.flag[Other(p)] && s'.pc == s.pc[p := a3b]) ||
+    (!s.flag[Other(p)] && s'.pc == s.pc[p := cs])
 }
 
-method a3b(p: Process, s: State, s': State) 
-requires p in P && Valid(s) && s.pc(p) == a3b)
+predicate stmt_a3b(p: Process, s: State, s': State) 
+requires ValidProcess(p) && Valid(s) && s.pc[p] == a3b
 {
-    (turn == Other(p) && s'.pc(p) == a3a) ||
-    (turn != Other(p) && s'.pc(p) == cs)
+    (s.turn == Other(p) && s'.pc == s.pc[p := a3a]) ||
+    (s.turn != Other(p) && s'.pc == s.pc[p := cs])
 }
 
-method cs(p:Process, s: State, s': State) 
-requires p in P && Valid(s) && s.pc(p) == cs)
+predicate stmt_cs(p:Process, s: State, s': State) 
+requires ValidProcess(p) && Valid(s) && s.pc[p] == cs
 {
-    s'.pc(p) == a4
+    s'.pc == s.pc[p := a4]
 }
 
-method a4(p: Process, s: State, s': State) 
-requires p in P && Valid(s) && s.pc(p) == a4) 
+predicate stmt_a4(p: Process, s: State, s': State) 
+requires ValidProcess(p) && Valid(s) && s.pc[p] == a4 
 {
-    s'.flag(p) == false &&
-    s'.pc(p) == a1
+    s'.flag == s.flag[p := false] &&
+    s'.pc == s.pc[p := a1]
 }
 
 // Mutual Exclusion
 lemma MutualExclusion(s: State, p: Process, q: Process)
 requires Valid(s)
-requires s.pc(p) == cs && s.pc(q) == cs
+requires s.pc[p] == cs && s.pc[q] == cs
 ensures p == q
 {
-    
+
 }
